rocq/README.md
@@ -1,51 +1,57 @@
 # Rocq Development overview
 
 - common
-  * common/core.v
-    Autosubst core definitions
-  * common/fintype.v
+  * [common.core](common/core.v)
+    Autosubst core definitions 
+  * [common.fintype](common/fintype.v)
     Autosubst fin type
-  * common/fin_util.v
+  * [common.fin_util](common/fin_util.v)
     Additional properties of fin type
-  * common/renaming.v
+  * [common.renaming](common/renaming.v)
     Language independent lemmas about renamings
-  * common/relations.v
+  * [common.relations](common/relations.v)x
     Multistep reduction
 
-- stlc Simply Typed Lambda Calculus
+- STLC: Simply Typed Lambda Calculus
   * stlc/syntax.sig
-  * stlc/syntax.v
-    Definition of the syntax
-  * stlc/typing.v
+    Autosubst input
+  * [stlc.syntax](stlc/syntax.v)
+    Definition of the syntax (generated)
+  * [stlc.typing](stlc/typing.v)
     Typing relation
-  * stlc/red.v
+  * [stlc.red](stlc/red.v)
     Small-step and big-step operational semantic
-  * stlc/safety.v
+  * [stlc.safety](stlc/safety.v)
     Preservation and progress
-  * stlc/small_step.v
+  * [stlc.small_step](stlc/small_step.v)
     Properties of small-step and multistep evaluation
-  * stlc/red_equiv.v
+  * [stlc.red_equiv](stlc/red_equiv.v)
     Equivalence between small-step and big-step
-  * stlc/soundness.v
-    Totality of big-step semantics
+  * [stlc.soundness](stlc/soundness.v)
+    Termination (totality) for of big-step semantics
 
-- rec Fine-grained CBV with recursive values and recursive types
-  * rec/syntax.sig
-  * rec/syntax.v
-    Term syntax
-  * rec/typesyntax.sig
-  * rec/typesyntax.v
-    Type syntax
-  * rec/reduction.v
-    Small-step operational semantics
-  * rec/typing.v
+- REC: Fine-grained CBV with recursive values and recursive types
+  * [syntax.sig](rec/syntax.sig)
+    Autosubst input for terms
+  * [rec.syntax](rec/syntax.v)
+    Generate term syntax
+  * [rec.typesyntax](rec/typesyntax.sig) 
+    Autosubst input for types
+  * [rec.typesyntax](rec/typesyntax.v)
+    Generate type syntax
+  * [rec.reduction](rec/reduction.v)
+    Small-step operational semantics. Includes some notes about Autosubst and 
+    various properties of the small-step relation.
+  * [rec.typing](rec/typing.v)
     Typing relation, preservation and progress proofs
-  * rec/semsound.v
+  * [rec.extensions](rec/extensions.v)
+    Derived syntactic forms for fine-grained CBV
+  * [rec.semsound](rec/semsound.v)
     Cannot show termination for multistep evaluation (incomplete proof)
-  * rec/iprop.v
-    downward-closed propositions indexed by steps
-  * rec/stepsLR.v
+  * [rec.iprop](rec/iprop.v)
+    propositions indexed by steps
+  * [rec.stepsLR](rec/stepsLR.v)
     Definition of step-indexed logical relation via strong induction (requires proof irrelevance)
-  * rec/steps.v
+  * [rec.steps](rec/steps.v)
     Proof of semantic soundness for step-indexed logical relation
 
